theories/theories/utp_sep_logic.thy
@@ -1,0 +1,31 @@
+theory utp_sep_logic
+imports "../utp_base"
+begin
+
+default_sort STORE_SORT
+
+abbreviation "heap \<equiv> MkPlainP ''heap'' True TYPE('m STORE) TYPE('m :: STORE_SORT)"
+
+lift_definition AssignS :: "(ADDR, 'm) PVAR \<Rightarrow> 'm WF_EXPRESSION \<Rightarrow> 'm WF_PREDICATE" ("[_] := _" [0, 190] 190) is
+"\<lambda> x e. {b. \<langle>b\<rangle>\<^sub>* heap\<acute> = (\<langle>b\<rangle>\<^sub>* heap)(\<langle>b\<rangle>\<^sub>*x :=\<^sub>s \<lbrakk>e\<rbrakk>\<^sub>eb)}" .
+
+term "[x] := v"
+
+
+(*
+definition fv :: "'a WF_ALPHA_PREDICATE \<Rightarrow> 'a VAR fset"
+where "fv(P) = pvar_alpha(\<alpha>(P))"
+
+definition prog_vars :: 
+  "'a VAR set \<Rightarrow> 
+   'a VAR set" ("pvar") where
+"pvar vs = vs \<inter> PROGRAM_VAR"
+
+lift_definition pvar_alpha :: 
+  "'a ALPHABET \<Rightarrow> 
+   'a ALPHABET" ("pvar\<^sub>\<alpha>") is pvar
+  by (simp add: fsets_def prog_vars_def)
+*)
+
+
+end
