theories/types/utp_memory.thy
@@ -1,0 +1,231 @@
+(******************************************************************************)
+(* Project: Unifying Theories of Programming in HOL                           *)
+(* File: utp_memory.thy                                                       *)
+(* Author: Simon Foster, University of York (UK)                              *)
+(******************************************************************************)
+
+header {* Simple memory model *}
+
+theory utp_memory
+imports 
+  "../core/utp_value"
+  "../poly/utp_poly_var"
+begin
+
+default_sort VALUE
+
+typedef ADDR = "UNIV :: nat set" ..
+
+declare Rep_ADDR [simp]
+declare Rep_ADDR_inverse [simp]
+declare Abs_ADDR_inverse [simplified, simp]
+
+class ADDR_SORT = VALUE +
+  fixes MkAddr   :: "ADDR \<Rightarrow> 'a"
+  and   DestAddr :: "'a \<Rightarrow> ADDR"
+  and   AddrType :: "'a UTYPE"
+  and   refs     :: "'a \<Rightarrow> ADDR fset"
+
+  assumes Inverse [simp] : "DestAddr (MkAddr x) = x"
+  and     AddrType_dcarrier: "dcarrier AddrType = range MkAddr"
+  and     refs_MkAddr: "refs (MkAddr x) = \<lbrace>x\<rbrace>"
+begin
+
+lemma Defined [defined]: "\<D> (MkAddr i)"
+  by (metis AddrType_dcarrier dcarrier_defined rangeI)
+
+lemma MkAddr_type [typing]: "MkAddr n : AddrType"
+  by (metis AddrType_dcarrier dcarrier_type rangeI)
+
+lemma MkAddr_dtype [typing]: "MkAddr n :! AddrType"
+  by (metis Defined MkAddr_type dtype_relI)
+
+lemma MkAddr_cases [elim]: 
+  "\<lbrakk> x :! AddrType; \<And> i. x = MkAddr i \<Longrightarrow> P \<rbrakk> \<Longrightarrow> P"
+  by (metis AddrType_dcarrier dtype_as_dcarrier image_iff)
+
+lemma MkAddr_inj_simp [simp]: 
+  "(MkAddr x = MkAddr y) \<longleftrightarrow> x = y"
+  by (metis Inverse)
+
+end
+
+instantiation ADDR :: DEFINED_NE
+begin
+definition "Defined_ADDR (x::ADDR) = True"
+instance 
+  by (intro_classes, auto simp add:Defined_ADDR_def)
+end
+
+lemma Defined_ADDR [defined]: "\<D> (x :: ADDR)" by (simp add:Defined_ADDR_def)
+
+defs (overloaded)
+  InjU_ADDR [inju]:  "InjU (x::ADDR) \<equiv> MkAddr x"
+  ProjU_ADDR [inju]: "ProjU (x::('a::ADDR_SORT)) \<equiv> DestAddr x"
+  TypeU_ADDR [simp]: "TypeU (x::ADDR itself) \<equiv> AddrType"
+
+lemma TypeUSound_ADDR [typing]: "TYPEUSOUND(ADDR, 'm :: ADDR_SORT)"
+  by (force simp add: typing defined inju)
+
+typedef 'a PADDR = "UNIV :: ADDR set" ..
+
+setup {*
+Adhoc_Overloading.add_variant @{const_name erase} @{const_name Rep_PADDR}
+*}
+
+definition prefs :: "'a \<Rightarrow> ('m::ADDR_SORT) itself \<Rightarrow> ADDR fset" where
+"prefs x t = refs (InjU x :: 'm)"
+
+(* Does this type need to avoid cyclicity? *)
+
+typedef ('m::ADDR_SORT) STORE = "{f :: (ADDR, 'm SIGTYPE) fmap. \<Union>\<^sub>f (refs `\<^sub>f sigvalue `\<^sub>f fran f) \<subseteq>\<^sub>f fdom f}"
+  by (rule_tac x="0" in exI, simp add:fran.rep_eq zero_fmap.rep_eq)
+
+setup_lifting type_definition_STORE
+
+(* notation Rep_STORE *)
+
+declare Rep_STORE [simp]
+declare Rep_STORE_inverse [simp]
+declare Abs_STORE_inverse [simp]
+
+lemma Rep_STORE_intro [intro!]:
+  "Rep_STORE x = Rep_STORE y \<Longrightarrow> x = y"
+  by (simp add:Rep_STORE_inject)
+
+lemma Rep_STORE_elim [elim]:
+  "\<lbrakk> x = y; Rep_STORE x = Rep_STORE y \<Longrightarrow> P \<rbrakk> \<Longrightarrow> P"
+  by (auto)
+
+lift_definition st_lookup :: "('m::ADDR_SORT) STORE \<Rightarrow> ADDR \<Rightarrow> 'm SIGTYPE" ("\<langle>_\<rangle>\<^sub>\<mu>") is "\<lambda> s k. the (Rep_fmap s k)" ..
+
+definition st_lookup_ty :: "('m::ADDR_SORT) STORE \<Rightarrow> 'a PADDR \<Rightarrow> 'a" where
+"st_lookup_ty s k = (if (TYPEU('a) = sigtype(\<langle>s\<rangle>\<^sub>\<mu> (k\<down>))) then ProjU(sigvalue(\<langle>s\<rangle>\<^sub>\<mu> (k\<down>))) else undefined)"
+
+lift_definition sdom :: "('m::ADDR_SORT) STORE \<Rightarrow> ADDR fset" is "fdom" ..
+lift_definition sran :: "('m::ADDR_SORT) STORE \<Rightarrow> 'm fset" is "\<lambda> x. (sigvalue `\<^sub>f fran x)" ..
+
+lift_definition srefs :: "('m::ADDR_SORT) STORE \<Rightarrow> ADDR fset" 
+is "\<lambda> f. \<Union>\<^sub>f (refs `\<^sub>f sigvalue `\<^sub>f fran f)" by (auto)
+
+lift_definition st_upd :: "('m::ADDR_SORT) STORE \<Rightarrow> ADDR \<Rightarrow> 'm SIGTYPE \<Rightarrow> 'm STORE" is
+"\<lambda> f k v. if (refs(sigvalue(v)) \<subseteq>\<^sub>f fdom(f) \<union>\<^sub>f \<lbrace>k\<rbrace>) then fmap_upd f k (Some v) else f"
+  apply (auto)
+  apply (metis (no_types) UN_I fupd_None_fran_subset less_eq_fset.rep_eq subsetD)
+done
+
+lemma st_upd_closed:
+  "\<lbrakk> refs(sigvalue(v)) \<subseteq>\<^sub>f sdom(s) \<union>\<^sub>f \<lbrace>k\<rbrace> \<rbrakk> \<Longrightarrow> Rep_STORE (st_upd s k v) = fmap_upd (Rep_STORE s) k (Some v)"
+  by (auto simp add: st_upd.rep_eq sdom.rep_eq)
+
+lemma st_lookup_upd_1: "refs(sigvalue(v)) \<subseteq>\<^sub>f sdom(s) \<union>\<^sub>f \<lbrace>k\<rbrace> \<Longrightarrow> \<langle>st_upd s k v\<rangle>\<^sub>\<mu> k = v"
+  by (auto simp add:st_lookup_def st_upd_closed)
+
+lemma st_lookup_upd_2: "\<lbrakk> refs(sigvalue(v)) \<subseteq>\<^sub>f sdom(s) \<union>\<^sub>f \<lbrace>k\<rbrace>; k \<noteq> k' \<rbrakk> \<Longrightarrow> \<langle>st_upd s k v\<rangle>\<^sub>\<mu> k' = \<langle>s\<rangle>\<^sub>\<mu> k'"
+  by (simp add:st_lookup_def st_upd_closed)
+
+definition st_upd_ty :: "('m::ADDR_SORT) STORE \<Rightarrow> 'a PADDR \<Rightarrow> 'a \<Rightarrow> 'm STORE" where
+"st_upd_ty s k v = st_upd s (k\<down>) (psigma v)"
+
+lemma st_lookup_upd_ty_1: 
+  fixes s :: "('m::ADDR_SORT) STORE" and k :: "'a PADDR"
+  assumes "TYPEUSOUND('a, 'm)" "prefs v TYPE('m) \<subseteq>\<^sub>f sdom(s) \<union>\<^sub>f \<lbrace>k\<down>\<rbrace>"
+  shows "st_lookup_ty (st_upd_ty s k v) k = v"
+  using assms by (simp add:st_lookup_ty_def st_upd_ty_def st_lookup_upd_1 prefs_def)
+
+lemma st_lookup_upd_ty_2: 
+  fixes s :: "('m::ADDR_SORT) STORE" and k :: "'a PADDR" and k' :: "'b PADDR"
+  assumes "TYPEUSOUND('a, 'm)" "prefs v TYPE('m) \<subseteq>\<^sub>f sdom(s) \<union>\<^sub>f \<lbrace>k\<down>\<rbrace>" "k\<down> = k'\<down>"
+  shows "st_lookup_ty (st_upd_ty s k v) k' = st_lookup_ty s k'"
+  using assms apply (simp add:st_lookup_ty_def st_upd_ty_def)
+oops
+
+instantiation STORE :: (ADDR_SORT) monoid_add
+begin
+
+lift_definition zero_STORE :: "'a STORE" is "fmempty"
+  by (simp add:fran.rep_eq zero_fmap.rep_eq)
+
+lift_definition plus_STORE :: "'a STORE \<Rightarrow> 'a STORE \<Rightarrow> 'a STORE" is 
+"\<lambda> x y. (x + y :: (ADDR, 'a SIGTYPE) fmap)"
+  apply (simp add:fran.rep_eq fdom.rep_eq plus_fmap.rep_eq)
+  apply (subgoal_tac "(\<Union>a\<in>ran (\<langle>fmap1\<rangle>\<^sub>m ++ \<langle>fmap2\<rangle>\<^sub>m). \<langle>refs(sigvalue(a))\<rangle>\<^sub>f) 
+                       \<subseteq> (\<Union>a\<in>ran \<langle>fmap1\<rangle>\<^sub>m. \<langle>refs(sigvalue(a))\<rangle>\<^sub>f) \<union> (\<Union>a\<in>ran \<langle>fmap2\<rangle>\<^sub>m. \<langle>refs(sigvalue(a))\<rangle>\<^sub>f)")
+  defer
+  apply (auto)[1]
+  apply (metis Un_iff ran_map_add_subset set_mp sup_set_def)
+  apply (auto)
+  apply (force)
+done
+
+instance
+  apply (intro_classes)
+  apply (auto simp add:zero_STORE.rep_eq plus_STORE.rep_eq)
+  apply (metis add_assoc)
+done
+
+end
+
+nonterminal supdbinds and supdbind
+
+syntax
+  "_supdbind" :: "['a, 'a] => supdbind"               ("(2_ :=\<^sub>s/ _)")
+  ""          :: "supdbind => supdbinds"              ("_")
+  "_supdbinds":: "[supdbind, supdbinds] => supdbinds" ("_,/ _")
+  "_SUpdate"  :: "['a, supdbinds] => 'a"              ("_/'((_)')" [1000, 0] 900)
+
+translations
+  "_SUpdate f (_supdbinds b bs)" == "_SUpdate (_SUpdate f b) bs"
+  "f(x:=\<^sub>sy)" == "CONST st_upd f x y"
+
+lemma srefs_subset_sdom: "srefs(\<Gamma>) \<subseteq>\<^sub>f sdom(\<Gamma>)"
+  apply (insert Rep_STORE[of "\<Gamma>"])
+  apply (auto simp add: sdom.rep_eq srefs.rep_eq)
+done
+
+class STORE_SORT = ADDR_SORT +
+  fixes MkStore   :: "'a STORE \<Rightarrow> 'a"
+  and   DestStore :: "'a \<Rightarrow> 'a STORE"
+  and   StoreType :: "'a UTYPE"
+
+  assumes Inverse [simp] : "DestStore (MkStore x) = x"
+  and     StoreType_dcarrier: "dcarrier StoreType = range MkStore"
+begin
+
+lemma Defined [defined]: "\<D> (MkStore i)"
+  by (metis StoreType_dcarrier dcarrier_defined rangeI)
+
+lemma MkStore_type [typing]: "MkStore n : StoreType"
+  by (metis StoreType_dcarrier dcarrier_type rangeI)
+
+lemma MkStore_dtype [typing]: "MkStore n :! StoreType"
+  by (metis Defined MkStore_type dtype_relI)
+
+lemma MkStore_cases [elim]: 
+  "\<lbrakk> x :! StoreType; \<And> i. x = MkStore i \<Longrightarrow> P \<rbrakk> \<Longrightarrow> P"
+  by (metis StoreType_dcarrier dtype_as_dcarrier image_iff)
+
+lemma MkStore_inj_simp [simp]: 
+  "(MkStore x = MkStore y) \<longleftrightarrow> x = y"
+  by (metis Inverse)
+
+end
+
+instantiation STORE :: (VALUE) DEFINED_NE
+begin
+definition "Defined_STORE (x::'a STORE) = True"
+instance 
+  by (intro_classes, auto simp add:Defined_STORE_def)
+end
+
+lemma Defined_STORE [defined]: "\<D> (x :: 'a STORE)" by (simp add:Defined_STORE_def)
+
+defs (overloaded)
+  InjU_STORE [inju]:  "InjU (x::('a::STORE_SORT) STORE) \<equiv> MkStore x"
+  ProjU_STORE [inju]: "ProjU (x::('a::STORE_SORT)) \<equiv> DestStore x"
+  TypeU_STORE [simp]: "TypeU (x::('a::STORE_SORT) STORE itself) \<equiv> StoreType"
+
+lemma TypeUSound_STORE [typing]: "TYPEUSOUND('m STORE, 'm :: STORE_SORT)"
+  by (force simp add: typing defined inju)
+
+end
